paxos/proof_agreement.dfy
@@ -141,26 +141,131 @@ c:Constants, ds:DistrSys, ds':DistrSys, actor:Id, recvIos:seq<Packet>, sendIos:s
     requires OneValuePerBallot(c, ds');
     ensures Agreement_Chosen_Inv_SomeValChosen(c, ds', b, v)
 {
+    AgreementChosenInv_NoneChosen_AccAction_NewChosenV_LargerBallotsPromiseQrms(c, ds, ds', actor, recvIos, sendIos, b, v);
+    assert LargerBallotsPromiseQrms(c, ds', b);  
+
+    
     assume LargerBallotAcceptors(c, ds', b, v);     // TODO: we need this
     assume LargerBallotAcceptMsgs(c, ds', b, v);     // TODO: we need this
 
+
     // Done
     AgreementChosenInv_NoneChosen_AccAction_NewChosenV_LargerBallotPromiseMsgs(c, ds, ds', actor, recvIos, sendIos, b, v);
-    assert LargerBallotPromiseMsgs(c, ds', b, v);  
-    
-
-    assume LargerBallotsPromiseQrms(c, ds', b);     // TODO: we need this
-
-    // Done
     AgreementChosenInv_NoneChosen_AccAction_NewChosenV_LargerBallotProposeMsgs(c, ds, ds', actor, recvIos, sendIos, b, v);
-    assert LargerBallotProposeMsgs(c, ds', b, v);
-
-    // Done
     AgreementChosenInv_NoneChosen_AccAction_NewChosenV_P2LeaderV(c, ds, ds', actor, recvIos, sendIos, b, v);
+    assert LargerBallotPromiseMsgs(c, ds', b, v);  
+    assert LargerBallotProposeMsgs(c, ds', b, v);
     assert LargerBallotPhase2LeadersV(c, ds', b, v);
 
     assert Agreement_Chosen_Inv_SomeValChosen(c, ds', b, v); 
 }
+
+
+lemma AgreementChosenInv_NoneChosen_AccAction_NewChosenV_LargerBallotsPromiseQrms(
+c:Constants, ds:DistrSys, ds':DistrSys, actor:Id, recvIos:seq<Packet>, sendIos:seq<Packet>, b:Ballot, v:Value)
+    requires Agreement_Chosen_Inv(c, ds)
+    requires ds'.WF(c) && Trivialities(c, ds')
+    requires Agreement_Chosen_Inv_Common(c, ds')
+    requires Next(c, ds, ds')
+    requires PaxosNextOneAgent(c, ds, ds', actor, recvIos, sendIos)
+    requires c.ValidAccId(actor)
+    requires recvIos[0].msg.Propose?
+    requires AcceptorAccept(ds.acceptors[actor.idx], ds'.acceptors[actor.idx], recvIos[0], sendIos);   
+    requires !SomeValueChosen(c, ds)
+    requires Chosen(c, ds', b, v)
+    ensures LargerBallotsPromiseQrms(c, ds', b)
+{
+    forall b' | BalLt(b, b') 
+    ensures LargerBalQuorumHasSeenB(c, ds', b, b')
+    {
+        forall qrm':set<Packet> | QuorumOfPromiseMsgs(c, ds', qrm', b') 
+        ensures QuorumHasSeenB(c, ds', qrm', b){
+            AgreementChosenInv_NoneChosen_AccAction_NewChosenV_LargerBallotsPromiseQrms_helper(c, ds, ds', actor, recvIos, sendIos, b, b', qrm', v);
+        }
+    }
+}
+
+lemma AgreementChosenInv_NoneChosen_AccAction_NewChosenV_LargerBallotsPromiseQrms_helper(
+c:Constants, ds:DistrSys, ds':DistrSys, actor:Id, recvIos:seq<Packet>, sendIos:seq<Packet>, b:Ballot, b':Ballot, qrm':set<Packet>, v:Value)
+    requires Agreement_Chosen_Inv(c, ds)
+    requires ds'.WF(c) && Trivialities(c, ds')
+    requires Agreement_Chosen_Inv_Common(c, ds')
+    requires Next(c, ds, ds')
+    requires PaxosNextOneAgent(c, ds, ds', actor, recvIos, sendIos)
+    requires c.ValidAccId(actor)
+    requires recvIos[0].msg.Propose?
+    requires AcceptorAccept(ds.acceptors[actor.idx], ds'.acceptors[actor.idx], recvIos[0], sendIos);   
+    requires !SomeValueChosen(c, ds)
+    requires Chosen(c, ds', b, v)
+    requires BalLt(b, b') 
+    requires QuorumOfPromiseMsgs(c, ds', qrm', b')
+    ensures QuorumHasSeenB(c, ds', qrm', b)
+{
+    /* Proof: Suppose otherwise. Then qrm' is in ds, and every Prom in qrm' has promised
+    * b', and saw < b. By PromisedImpliesNoMoreAccepts, this means that no Accept(b) messages
+    * from any acceptor in qrm'.
+    * Call the set of acceptors that chose (b, v) in ds' as qrm. Then qrm and qrm' must be disjoint, 
+    * and their union is the set of all acceptors, and qrm is size f. 
+    * Now consider the actor taking a step: 
+    *   1. If actor is in qrm', it can't accept (b, v). Hence (b,v) not chosen in ds'. C!
+    *   2. If actor is in qrm, |qrm| remains f in ds'. C!
+    */
+    if !QuorumHasSeenB(c, ds', qrm', b) {
+        forall prom | prom in qrm' ensures BalLt(prom.msg.vb.b, b) {}
+        lemma_NoPromiseSentInAcceptStep(c, ds, ds', actor, recvIos, sendIos);
+        assert QuorumOfPromiseMsgs(c, ds, qrm', b');
+        
+        // Get set of acceptors that promised b' (and not seen b) in ds
+        var accs_that_promised := extractPacketSources(qrm');
+        assert |accs_that_promised| >= c.f + 1;
+
+        // Get set of acceptors that voted to choose (b, v) in ds
+        var qrm :| QuorumOfAcceptMsgs(c, ds', qrm, b) && AccPacketsHaveValueV(qrm, v);
+        var new_accept_pkt := lemma_NewChosenImpliesOneNewAcceptPacket(c, ds, ds', actor, recvIos, sendIos, b, v);
+        var pre_qrm := qrm - {new_accept_pkt};   // set without the latest Accept from ds->ds' actor.
+        assert SetOfAcceptMsgs(c, ds, pre_qrm, b);
+        lemma_Set_MinusElem(qrm, new_accept_pkt, |qrm|);
+        var accs_that_accepted := extractPacketSources(pre_qrm);
+        assert |accs_that_accepted| >= c.f;
+
+        // Show that accs_that_promised && accs_that_accepted are disjoint;
+        // use PromisedImpliesNoMoreAccepts
+        forall id | id in accs_that_promised 
+        ensures id !in accs_that_accepted
+        {
+            var prom :| prom in qrm' && prom.src == id;
+            forall accp | accp in qrm 
+            ensures accp.src != id
+            {
+                if accp.src == id {      
+                    assert !BalLtEq(accp.msg.bal, prom.msg.vb.b);
+                    lemma_BalLtSynonyms(b, b');
+                    assert !BalLtEq(prom.msg.bal, accp.msg.bal);
+                    assert false;
+                }
+            }
+        }
+        lemma_Set_DisjointSets(accs_that_promised, accs_that_accepted);
+
+        // Consider the current actor taking a step
+        lemma_IdSetCover(c, ds, accs_that_promised, accs_that_accepted, actor);
+        if actor in accs_that_promised {
+            assert BalLtEq(b', ds.acceptors[actor.idx].promised);   // by PromiseMsgImpliesPromised
+            lemma_BalLtTransitivity1(b, b', ds.acceptors[actor.idx].promised);
+            lemma_NewChosenImpliesIncomingProposalBV(c, ds, ds', actor, recvIos, sendIos, b, v);
+            assert !AcceptorAccept(ds.acceptors[actor.idx], ds'.acceptors[actor.idx], recvIos[0], sendIos); 
+            assert false;
+        } else {
+            assert actor in accs_that_accepted;
+            var p :| p in pre_qrm && p.src == actor && isAcceptPkt(ds, p) && p.msg.bal == b;
+            lemma_NewChosenImpliesIncomingProposalBV(c, ds, ds', actor, recvIos, sendIos, b, v);
+            assert sendIos[0] == p;
+            assert ds'.network.sentPackets == ds.network.sentPackets;
+            assert false;       // violates lemma_NewChosenImpliesOneNewAcceptPacket
+        }
+    }
+}
+
 
 
 lemma AgreementChosenInv_NoneChosen_AccAction_NewChosenV_LargerBallotPromiseMsgs(
@@ -237,10 +342,8 @@ c:Constants, ds:DistrSys, ds':DistrSys, actor:Id, recvIos:seq<Packet>, sendIos:s
     requires AcceptorAccept(ds.acceptors[actor.idx], ds'.acceptors[actor.idx], recvIos[0], sendIos);   
     requires !SomeValueChosen(c, ds)
     requires Chosen(c, ds', b, v)
-    requires OneValuePerBallot(c, ds')
     requires LargerBallotsPromiseQrms(c, ds', b)
     requires LargerBallotPromiseMsgs(c, ds', b, v)
-    requires b != Bottom
     ensures LargerBallotPhase2LeadersV(c, ds', b, v)
 {
     forall l_idx |  && c.ValidLdrIdx(l_idx) 
